lib/AbsDen/Laws.lean
@@ -107,24 +107,24 @@ abbrev DefiHeap := FinMap Addr DefiD
 abbrev DefiHeap.μ (μ : DefiHeap) : Heap := FinMap.map_with_key (fun a d => memo a (next[]. d.d)) μ
 abbrev DefiHeap.dom (μ : DefiHeap) : Set Addr := fun a => a ∈ μ.keys
 
-def T.steps (ev : List Event) (t : T (Heap × Value)) : T (Heap × Value) :=
-  List.foldr (fun e t => T.step e (next[]. t)) t ev
+def Trace.steps (ev : List Event) (t : T (Heap × Value)) : T (Heap × Value) :=
+  List.foldr (fun e t => Trace.step e (next[]. t)) t ev
 @[simp]
-lemma T.steps_nil : T.steps [] d = d := by unfold T.steps; simp
+lemma Trace.steps_nil : Trace.steps [] d = d := by unfold Trace.steps; simp
 @[simp]
-lemma T.steps_cons : T.steps (e::ev) d = T.step e (next[]. T.steps ev d) := by unfold T.steps; simp
+lemma Trace.steps_cons : Trace.steps (e::ev) d = Trace.step e (next[]. Trace.steps ev d) := by unfold Trace.steps; simp
 
 structure BalancedExec (d₁ : DefiD) (μ₁ : DefiHeap) (d₂ : DefiD) (μ₂ : DefiHeap) where
   mk ::
   events : List Event
   is_value : d₂.e.is_value
-  property : d₁.d.f μ₁.μ = T.steps events (d₂.d.f μ₂.μ)
+  property : d₁.d.f μ₁.μ = Trace.steps events (d₂.d.f μ₂.μ)
 
 structure StuckExec (d₁ : DefiD) (μ₁ : DefiHeap) where
   mk ::
   events : List Event
   μ₂ : DefiHeap
-  property : d₁.d.f μ₁.μ = T.steps events ((Domain.stuck : D).f μ₂.μ)
+  property : d₁.d.f μ₁.μ = Trace.steps events ((Domain.stuck : D).f μ₂.μ)
 
 notation:max "<" e₁:max "," μ₁:max ">⇓<" e₂:max "," μ₂:max ">" => BalancedExec e₁ μ₁ e₂ μ₂
 
@@ -132,7 +132,7 @@ lemma eval_deterministic : <⟨e,ρ₁⟩,μ₁>⇓<⟨e₂,ρ₂⟩,μ₂> → 
   sorry
 
 lemma ne_steps_fun_stuck :
-  ∀ ev₁ ev₂ μ₁ μ₂ g, T.steps ev₁ ((instDomainD.fn g).f μ₁) ≠ T.steps ev₂ (instDomainD.stuck.f μ₂)
+  ∀ ev₁ ev₂ μ₁ μ₂ g, Trace.steps ev₁ ((instDomainD.fn g).f μ₁) ≠ Trace.steps ev₂ (instDomainD.stuck.f μ₂)
 := by
   intro ev₁ ev₂ _ _ _
   induction ev₁ generalizing ev₂
@@ -176,13 +176,23 @@ inductive HeapProgression : DefiHeap → DefiHeap → Prop where
 notation μ₁ " ↝ " μ₂ => HeapProgression μ₁ μ₂
 
 lemma eval_progesses_heap : <⟨e,ρ₁⟩,μ₁>⇓<⟨v,ρ₂⟩,μ₂> → μ₁ ↝ μ₂ := gfix fun hind hevals => by
-  have ⟨events, ⟨x,e',hval⟩, property⟩ := hevals
+  have ⟨events, ⟨z,e',hval⟩, property⟩ := hevals
   simp at hval
   rw[hval] at property
-  unfold DefiD.d evalByNeed eval at *
-  simp at *
+  unfold DefiD.d evalByNeed eval at property
+  simp at property
   cases e
-  case var x => simp at property; split at property; cases events; simp at *;
+  case var x =>
+    simp at property
+    split at property
+    next h =>
+      obtain ⟨a,hfetch⟩ := ρ₁.property x h
+      generalize ρ₁.val[x] = entry at *
+      simp at property
+      cases events;
+      · simp at property
+      · simp at property; rw[hfetch] at property; unfold fetch at property; simp at property; rw[Later.unsafeFlip_eq] at property; split at property;  sorry
+    next => absurd property.symm; apply ne_steps_fun_stuck events ([])
 
 lemma abs_ByNeed_interpretation' [AbstractByNeedDomain A] : αS A (evalByNeed e ρ) μ ≤ eval e := sorry
 theorem abs_ByNeed_interpretation [AbstractByNeedDomain A] : αS A (evalByNeed e) ≤ eval e := sorry
